\documentclass{article}
\usepackage{epsfig}
\pagestyle{empty}
\begin{document}
\[ U = \sum_{ij} \varphi(r_{ij}) + \sum_i F({\bar\rho_i}) \]
\pagebreak

$\varphi_{ij}$
\pagebreak

$F(\bar\rho)$
\pagebreak

$\bar\rho$
\pagebreak

\[ \bar\rho_i = \sum_j \rho_j(r_{ij}) \]
\pagebreak

${\bf F}_i$
\pagebreak

\begin{eqnarray*} {\bf F}_i & = & -\nabla_i \sum_{jk} U(r_{jk})\\ & = & - \sum_j\left\{ \varphi'(r_{ij}) + [F'(\bar\rho_i) + F'(\bar\rho_j)]\rho'(r_{ij}) \right\} \hat{r}_{ij} \end{eqnarray*}
\pagebreak

$\hat{r}_{ij}$
\pagebreak

$ F'(\bar\rho) $
\pagebreak

$ \bar\rho $
\pagebreak

$ F'(\bar\rho_j) $
\pagebreak

$ \bar\rho_j $
\pagebreak

$[x_0, x_n]$
\pagebreak

$x_n = n*dx$
\pagebreak

\[phi = Z(r) * Z(r) / r\]
\pagebreak

\[ E_{tot} = \sum_{ij} U_{LJ}(r_{ij}) \]
\pagebreak

\[ U_{LJ}(r_{ij}) = 4 \epsilon \left\{ \left(\frac{\sigma}{r_{ij}}\right)^{12} - \left(\frac{\sigma}{r_{ij}}\right)^6 \right\} \]
\pagebreak

$\epsilon$
\pagebreak

$\sigma$
\pagebreak

\[ F_i = -\nabla_i \sum_{jk} U_{LJ}(r_{jk}) \]
\pagebreak

\begin{eqnarray*} F_i &=& - \sum_j U'_{LJ}(r_{ij})\hat{r}_{ij}\\ &=& \sum_j 24 \frac{\epsilon}{r_{ij}} \left\{ 2 \left(\frac{\sigma}{r_{ij}}\right)^{12} - \left(\frac{\sigma}{r_{ij}}\right)^6 \right\} \hat{r}_{ij} \end{eqnarray*}
\pagebreak

\end{document}
